smtlink/test-all.lisp
@@ -1,77 +1,112 @@
 ;; test cases
-:logic
+(in-package "ACL2")
+(include-book "./SMT-connect")
+
+(logic)
+:set-state-ok t
 
 ;; test0
 (defconst *a* 1)
-(defun bar1 (x) (* 2 x))
+(defun bar0 (x) (* 2 x))
 
 ;; a very simple theorem
 (defthm test0
   (implies (and (and (rationalp x)) (and))
-	   (equal (+ x x) (* *a* (bar1 x))))
+	   (equal (+ x x) (* *a* (bar0 x))))
   :hints
-            (("Goal"
-              :clause-processor
-              (my-clause-processor clause
-				   '( (:expand (bar1) 1)
-				      (:python-file "test0")
-				      (:let ())
-				      (:hypothesize ()))
-				      ))))
+  (("Goal"
+    :clause-processor
+    (my-clause-processor clause
+			 '( (:expand (bar0))
+			   (:python-file "test0")
+			   (:let ())
+			   (:hypothesize ()))
+			 ))))
 
 ;; test1
 (defun foo1 (x y) (* x (+ 1 y)))
 
 ;; very first piece of test case
-(thm (implies (and (and (rationalp x)
-			(integerp y)
-			(integerp z))
-		   (and (not (<= x 0))
-			(equal z (+ 3/2 4))
-			(or (> x y) (> x (+ y 40/3)))))
-	      (> (foo1 x (foo1 x z)) (foo1 x y)))
-     :hints
-            (("Goal"
-              :clause-processor
-              (my-clause-processor clause
-				   '( (:expand (foo1) 2)
-				      (:python-file "test1")
-				      (:let ())
-				      (:hypothesize ()))))))
-
-;; test2
-(defun foo (x) (+ x 3))
-(defun bar (y) (* 2 (foo y)))
-
-(defthm test2
-  (implies (and (and (rationalp y))
-		(and (> y 1)))
-	   (> (bar (foo y)) 12))
+(defthm test1 (implies (and (and (rationalp x)
+				 (integerp y)
+				 (integerp z))
+			    (and (not (<= x 0))
+				 (equal z (+ 3/2 4))
+				 (or (> x y) (> x (+ y 40/3)))))
+		       (> (foo1 x (foo1 x z)) (foo1 x y)))
   :hints
   (("Goal"
     :clause-processor
     (my-clause-processor clause
-			 '( (:expand (foo bar) 5)
+			 '( (:expand (foo1))
+			   (:python-file "test1")
+			   (:let ())
+			   (:hypothesize ()))))))
+
+;; test2
+(defun foo2 (x) (+ x 3))
+(defun bar2 (y) (* 2 (foo2 y)))
+
+(defthm test2
+  (implies (and (and (rationalp y))
+		(and (> y 1)))
+	   (> (bar2 (foo2 y)) 12))
+  :hints
+  (("Goal"
+    :clause-processor
+    (my-clause-processor clause
+			 '( (:expand (foo2 bar2))
 			    (:python-file "test2")
 			    (:let ())
 			    (:hypothesize ()))))))
 
 ;; test3
-(defun foo2 (x args) (+ x (nth 0 args) (nth 1 args)))
+(defun foo3 (x args) (+ x (nth 0 args) (nth 1 args)))
 
-(defthm test4
+(defthm test3
   (implies (and (and (rationalp x)
 		     (integerp i)
 		     (integerp j))
 		(and (> x 0)
 		     (> i 0)
 		     (> j 0)))
-	   (> (foo2 x '(i j)) 0))
+	   (> (foo3 x '(i j)) 0))
   :hints
   (("Goal"
     :clause-processor
     (my-clause-processor clause
-			 '( (:expand (foo2) 1)
+			 '( (:expand (foo3))
 			    (:python-file "test3")
+			    (:let ())
+			    (:hypothesize ()))))))
+
+;; test4
+;; x^2 + y^2 >= 2xy
+;; a(x,y) = x*y
+;; b(x) = 2*x = (a 2 x)
+;; c(x,y) = x+y
+;; d(x) = x^2 = (a x x)
+;; e(x) = -x
+;; f(x,y) = x-y = (c x -y) = (c x (e y))
+(defun a4 (x y) (* x y))
+(defun b4 (x) (a4 2 x))
+(defun c4 (x y) (+ x y))
+(defun d4 (x) (a4 x x))
+(defun e4 (x) (- x))
+(defun f4 (x y) (c4 x (e4 y)))
+
+(defthm test4
+    (implies (and (and (rationalp a)
+		       (rationalp b))
+		  (and))
+	     (>= (f4 (d4 (c4 a b))
+		     (a4 (b4 a) b))
+		 (a4 (b4 a) b)))
+  :hints
+  (("Goal"
+    :clause-processor
+    (my-clause-processor clause
+			 '( (:expand (a4 b4 c4 d4 e4 f4))
+			    (:python-file "test4")
 			    (:let ())
 			    (:hypothesize ()))))))
