smtlink/SMT-function.lisp
@@ -1,9 +1,7 @@
 ;; SMT-function
 (in-package "ACL2")
 (include-book "str/top" :dir :system)
-
-:set-state-ok t
-:set-ignore-ok t
+(include-book "./helper")
 
 ;; create-name
 (defun create-name (num)
@@ -80,7 +78,7 @@
 ;; e.g.(defun double (x y) (+ (* 2 x) y))
 ;;     (double a b) -> (let ((var1 a) (var2 b)) (+ (* 2 var1) var2))
 ;;     (double a b) -> ((lambda (var1 var2) (+ (* 2 var1) var2)) a b)
-(defun expand-a-fn (fn num state)
+(defun expand-a-fn (fn fn-waiting fn-extended num state)
   "expand-a-fn: expand an expression with a function definition, num should be accumulated by 1. fn should be stored as a symbol"
   (let ((formal (cdr (cadr (meta-extract-formula fn state))))
 	;; the third element is the formals
@@ -90,7 +88,10 @@
     (mv-let (var-list num1)
 	    (make-var-list formal num)
 	    (mv (list 'lambda (assoc-fetch-value var-list)
-		      (set-fn-body body var-list))  num1))))
+		      (set-fn-body body var-list))
+		(my-delete fn-waiting fn)
+		(cons fn fn-extended)
+		num1))))
 
 ;; lambdap
 (defun lambdap (expr)
@@ -98,8 +99,8 @@
   (if (not (equal (len expr) 3))
       nil
       (let ((lambdax (car expr))
-	    (formals (cadr expr))
-	    (body (caddr expr)))
+	    (formals (cadr expr)))
+	    ;;(body (caddr expr)))
 	(if (and (equal lambdax 'lambda)
 		 (listp formals)) ;; I can add a check for no
 	                          ;; occurance of free variable in the future
@@ -108,53 +109,85 @@
 
 (mutual-recursion
  ;; expand-fn-help-list
- (defun expand-fn-help-list (expr fn-lst num state)
+ (defun expand-fn-help-list (expr fn-lst fn-waiting fn-extended num state)
    "expand-fn-help-list"
+   (declare (xargs :measure (list (len fn-waiting) (acl2-count expr))))
    (if (endp expr)
        (mv nil num)
      (mv-let (res-expr1 res-num1)
-	     (expand-fn-help (car expr) fn-lst num state)
+	     (expand-fn-help (car expr) fn-lst fn-waiting fn-extended num state)
 	     (mv-let (res-expr2 res-num2)
-		     (expand-fn-help-list (cdr expr) fn-lst res-num1 state)
+		     (expand-fn-help-list (cdr expr) fn-lst fn-waiting fn-extended res-num1 state)
 		     (mv (cons res-expr1 res-expr2) res-num2)))))
 
  ;; expand-fn-help
- (defun expand-fn-help (expr fn-lst num state)
+ ;; This function should keep three lists of function names.
+ ;   First one stores all functions possible for expansion.
+ ;   Second one is for functions to be expanded
+ ;   and the third one is for functions already expanded.
+ ;; They should be updated accordingly:
+ ;   when one function is expanded along a specific path
+ ;   that function should be deleted from fn-waiting and added
+ ;   into fn-expanded.
+ ;; Resursion detection:
+ ;   When one function call is encountered
+ ;   we want to make sure that function is valid for expansion
+ ;   by looking at fn-lst. Then we expand it, delete it from
+ ;   fn-waiting and add it onto fn-expanded. The we want to make
+ ;   sure that fn-waiting and fn-expaned is changing as we walk
+ ;   through the tree of code.
+ ;; Another way of recursion detection:
+ ;   One might want to use this simpler way of handling recrusion
+ ;   detection. We note the length of fn-lst, then we want to
+ ;   count down the level of expansion. Any path exceeding this
+ ;   length is a sign for recursive call. 
+ (defun expand-fn-help (expr fn-lst fn-waiting fn-extended num state)
    "expand-fn-help: expand an expression"
-   (cond ((atom expr)
+   (declare (xargs :measure (list (len fn-waiting) (acl2-count expr))))
+   (cond ((atom expr) ;; base case, when expr is an atom
  	  (mv expr num))
- 	 ((consp expr) ;; expr is a function application
- 	  (b*
- 	   ((fn0 (car expr)) ;; function name
- 	    (params (cdr expr)) ;; function parameters
- 	    ((mv fn num2)
- 	     (cond
- 	       ((and (atom fn0) (exist fn0 fn-lst)) ;; function exists in the list
- 		(expand-a-fn fn0 num state)) ;; expand a function
- 	       ((lambdap fn0) ;; function is a lambda expression
- 		(let ((lambdax fn0) (params (cdr expr)))
-  		  (let ((formals (cadr lambdax)) (body (caddr lambdax)))
-  		    (mv-let (body-expr body-num)
-  			    (expand-fn-help body fn-lst num state)
- 			    (mv (list 'lambda formals body-expr) body-num)))))
- 	       ((and (not (lambdap fn0)) (consp fn0))
- 		(expand-fn-help fn0 fn-lst num state)) ;; for handling lists
- 	       ((atom fn0)
- 		(mv fn0 num))
- 	       (t (prog2$ 
- 		   (cw "Error(function): not a valid function application ~q0" expr)
- 		   (mv expr num))))))
- 	   (mv-let (res num3)
- 		   (expand-fn-help-list params fn-lst num2 state)
-		   (mv-let (res2 num4)
-			   (expand-fn-help fn fn-lst num3 state)
-			   (mv (cons res2 res) num4)))))
- 	 (t (prog2$ (cw "Error(function): strange expression == ~q0" expr)
+	 ((consp expr)
+	  (let ((fn0 (car expr)) (params (cdr expr)))
+	    (cond
+	      ((lambdap fn0) ;; function is a lambda expression, expand the body
+	       (let ((lambdax fn0) (params (cdr expr)))
+		 (let ((formals (cadr lambdax)) (body (caddr lambdax)))
+		   (mv-let (res num2)
+			   (expand-fn-help body fn-lst fn-waiting fn-extended num state)
+			   (mv-let (res2 num3)
+				   (expand-fn-help-list params fn-lst fn-waiting fn-extended num2 state)
+				   (mv (cons (list 'lambda formals res) res2) num3))))))
+	      ((and (not (lambdap fn0)) (consp fn0)) ;; for handling lists 
+	       (mv-let (res num2)
+		       (expand-fn-help fn0 fn-lst fn-waiting fn-extended num state)
+		       (mv-let (res2 num3)
+			       (expand-fn-help-list params fn-lst fn-waiting fn-extended num2 state)
+			       (mv (cons res res2) num3))))
+	      ((and (atom fn0) (exist fn0 fn-lst)) ;; function exists in the list
+	       (if (and (exist fn0 fn-waiting) (not (exist fn0 fn-extended))) ;; if fn0 exist in waiting list and not in extended list
+		   (mv-let (res fn-w-1 fn-e-1 num2)
+			   (expand-a-fn fn0 fn-waiting fn-extended num state) ;; expand a function
+			   (mv-let (res2 num3)
+				   (expand-fn-help res fn-lst fn-w-1 fn-e-1 num2 state)
+				   (mv-let (res3 num4)
+					   (expand-fn-help-list params fn-lst fn-waiting fn-extended num3 state)
+					   (mv (cons res2 res3) num4))))
+		   (prog2$ (cw "Error(function): possible recursive function call detected: ~q0" fn0)
+			   (mv expr num))))
+	      ((and (consp expr) (atom (car expr))) ;; when expr is a un-expandable function
+	       (mv-let (res num2)
+		       (expand-fn-help-list (cdr expr) fn-lst fn-waiting fn-extended num state)
+		       (mv (cons (car expr) res) num2)))
+	      (t (prog2$ 
+ 		   (cw "Error(function): not a valid function application ~q0" fn0)
+ 		   (mv expr num)))
+	      )))
+	 (t (prog2$ (cw "Error(function): strange expression == ~q0" expr)
  		    (mv expr num)))))
 )
 ;; expand-fn
-(defun expand-fn (expr fn-lst level state)
+(defun expand-fn (expr fn-lst state)
   "expand-fn: takes an expr and a list of functions, unroll the expression. fn-lst is a list of possible functions for unrolling."
   (mv-let (res-expr res-num)
-	  (expand-fn-help expr fn-lst 0 state)
+	  (expand-fn-help expr fn-lst fn-lst nil 0 state)
 	  (prog2$ (cw "The final index number: ~q0" res-num) res-expr)))
