smtlink/SMT-translator.lisp
@@ -91,42 +91,42 @@
 	    (cons #\Newline (translate-constant-list (cdr const-list))))
     nil))
 
-;; check-const
-(defun check-const (expr)
-  "check-const: check to see if an expression is a constant"
-  (if (and (atom expr)
-	   (let ((expr-list (coerce (symbol-name expr) 'list)))
-	     (and (equal #\* (car expr-list))
-		  (equal #\* (nth (1- (len expr-list)) expr-list)))))
-      t
-    nil))
+;; ;; check-const
+;; (defun check-const (expr)
+;;   "check-const: check to see if an expression is a constant"
+;;   (if (and (atom expr)
+;; 	   (let ((expr-list (coerce (symbol-name expr) 'list)))
+;; 	     (and (equal #\* (car expr-list))
+;; 		  (equal #\* (nth (1- (len expr-list)) expr-list)))))
+;;       t
+;;     nil))
 
-;; get-constant-list-help
-(defun get-constant-list-help (expr const-list)
-  "get-constant-list-help: check all constants in a clause"
-  (cond
-    ( (consp expr)
-      (let ((const-list-2 (get-constant-list-help (car expr) const-list)))
-	(get-constant-list-help (cdr expr) const-list-2))
-    )
-    ( (check-const expr)
-      (mv-let (keyword name value)
-	      (pe expr) ;; pe will not be working for this
-	      (cons (list expr (translate-number value)) const-list))
-      )
-    ( (atom expr)
-      (get-constant-list-help (cdr expr) const-list)
-      )
-    ( t
-      const-list
-      )
-    )
-  )
+;; ;; get-constant-list-help
+;; (defun get-constant-list-help (expr const-list)
+;;   "get-constant-list-help: check all constants in a clause"
+;;   (cond
+;;     ( (consp expr)
+;;       (let ((const-list-2 (get-constant-list-help (car expr) const-list)))
+;; 	(get-constant-list-help (cdr expr) const-list-2))
+;;     )
+;;     ( (check-const expr)
+;;       (mv-let (keyword name value)
+;; 	      (pe expr) ;; pe will not be working for this
+;; 	      (cons (list expr (translate-number value)) const-list))
+;;       )
+;;     ( (atom expr)
+;;       (get-constant-list-help (cdr expr) const-list)
+;;       )
+;;     ( t
+;;       const-list
+;;       )
+;;     )
+;;   )
 
-;; get-constant-list
-(defun get-constant-list (expr)
-  "get-constant-list: get the list of constants in an associate list"
-  (get-constant-list-help expr '()))
+;; ;; get-constant-list
+;; (defun get-constant-list (expr)
+;;   "get-constant-list: get the list of constants in an associate list"
+;;   (get-constant-list-help expr '()))
 
 
 ;; ----------------------- translate-declaration ---------------------------:
@@ -233,7 +233,7 @@
 ;; translate-SMT-formula
 (defun translate-SMT-formula (formula)
   "translate-SMT-formula: translate a SMT formula into its Z3 code"
-  (let ((const-list (car formula))
+  (let (;(const-list (car formula))
 	(decl-list (cadr formula))
 	(hypo-list (caddr formula))
 	(concl-list (cadddr formula)))
