smtlink/helper.lisp
@@ -5,3 +5,13 @@
 (defun my-last (listx)
  "my-last: fetch the last element from list"
   (car (last listx)))
+
+;; my-delete
+(defun my-delete (listx elem)
+  "my-delete: delete an element from the list. If there're duplicates, this function deletes the first one in the list."
+  (if (endp listx) ;; elem does not exist in the list
+      listx
+      (if (equal (car listx) elem)
+	  (cdr listx)
+	  (cons (car listx)
+		(my-delete (cdr listx) elem)))))
